x86/Asm.v
@@ -1141,32 +1141,45 @@ Definition funsig (fd: fundef) :=
   | External ef => ef_sig ef
   end.
 
-Definition set_arg (rs: regset) (l: loc) (v: val) : regset :=
+Definition make_arg (rs: regset) (m: mem) (l: loc) (v: val) : option (regset * mem) :=
   match l with
-  | R r => rs # (preg_of r) <- v
-  | S _ _ _ => rs
+  | R r => Some (rs # (preg_of r) <- v, m)
+  | S _ ofs ty =>
+      let bofs := (Stacklayout.fe_ofs_arg + 4 * ofs)%Z  in
+      match Mem.storev (chunk_of_type ty) m (Val.offset_ptr (rs (IR SP)) (Ptrofs.repr bofs)) v with
+      | Some m' => Some (rs, m')
+      | None => None
+      end
   end.
 
-Fixpoint set_arguments (rs: regset) (al: list (rpair loc)) (lv: list val) : option regset :=
+Fixpoint make_arguments (rs: regset) (m: mem) (al: list (rpair loc)) (lv: list val) :
+  option (regset * mem) :=
   match al, lv with
   | a :: al', v :: lv' =>
-    match set_arguments rs al' lv' with
-    | Some rs' =>
+    match make_arguments rs m al' lv' with
+    | Some (rs', m') =>
       match a with
-      | One l => Some (set_arg rs' l v)
+      | One l => make_arg rs' m' l v
       | Twolong hi lo =>
         match v with
         | Vlong v' =>
-            Some (set_arg (set_arg rs' hi (Vint (Int64.hiword v'))) lo (Vint (Int64.loword v')))
+          match make_arg rs' m' hi (Vint (Int64.hiword v')) with
+          | Some (rs'', m'') => make_arg rs'' m'' lo (Vint (Int64.loword v'))
+          | None => None
+          end
         | Vundef =>
-            Some (set_arg (set_arg rs' hi Vundef) lo Vundef)
+          match make_arg rs' m' hi Vundef with
+          | Some (rs'', m'') => make_arg rs'' m'' lo Vundef
+          | None => None
+          end
         | _ => None
         end
       end
     | _ => None
     end
-  | _, _ => Some rs
-  end.
+  | nil, nil => Some (rs, m)
+  | _, _ => None
+ end.
 
 Inductive entry_point (ge:genv): mem -> state -> val -> list val -> Prop:=
 | INIT_CORE:
@@ -1174,11 +1187,11 @@ Inductive entry_point (ge:genv): mem -> state -> val -> list val -> Prop:=
       let rs0 :=
         (Pregmap.init Vundef)
         # PC <- (Vptr b Ptrofs.zero) 
-        # RA <- Vzero
-        # RSP <- Vnullptr in
+        # RA <- Vnullptr
+        # RSP <- sp in
       Genv.find_funct_ptr ge b = Some f ->
-      set_arguments rs0 (loc_arguments (funsig f)) args = Some rs ->
-      entry_point ge m (State rs m) (Vptr b (Ptrofs.of_ints Int.zero)) args.
+      make_arguments rs0 m0 (loc_arguments (funsig f)) args = Some (rs, m) ->
+      entry_point ge m0 (State rs m) (Vptr b (Ptrofs.of_ints Int.zero)) args.
 
  Definition get_extcall_arg (rs: regset) (m: mem) (l: Locations.loc) : option val :=
  match l with
